re-added 'global pick_sp' version of exec in same file. will prove it equivalent to 'local' version

bedrock2/src/bedrock2/Semantics.v
@@ -280,6 +280,10 @@ Section semantics.
   End WithMemAndLocals.
 End semantics.
 
+Definition PickSp {width: Z}{BW: Bitwidth width}{word: word.word width}{mem: map.map word byte} : Type :=
+  trace -> word.
+Existing Class PickSp.
+
 Module exec. Section WithEnv.
   Context {width: Z} {BW: Bitwidth width} {word: word.word width} {mem: map.map word byte}.
   Context {locals: map.map String.string word}.
@@ -291,117 +295,132 @@ Module exec. Section WithEnv.
 
   Implicit Types post : trace -> io_trace -> mem -> locals -> metrics -> Prop. (* COQBUG(unification finds Type instead of Prop and fails to downgrade *)
 
-  (*maybe input trace should be entire trace so far, but trace in postcondition should just be trace accumulated during execution.*)
-  Inductive exec :
-    (trace -> word) -> cmd -> trace -> io_trace -> mem -> locals -> metrics ->
+  (*I really want to do the semantics like this:
+    cmd -> io_trace -> mem -> locals -> metrics ->
+    (trace -> io_trace -> mem -> locals -> metrics -> Prop) -> Prop.
+    But it would be ugly.  Using app, screwing up simple postconditions
+    (e.g., in seq case) in semantics.
+    
+    So I suppose I'll do 
+    cmd -> trace -> io_trace -> mem -> locals -> metrics ->
+    (trace -> io_trace -> mem -> locals -> metrics -> Prop) -> Prop.
+    
+    Then we can state a lemma, saying that exec c nil t m l mc post -> exec c k t m l mc (fun k' => post (k' ++ k)).
+    Then use that wherever we want, and it's *almost* like leakage trace isn't passed as a parameter to exec.
+    Still ugly though.  But better?  No, not really.  Would be horribly obnoxious to apply that lemma.  Hm.
+
+    I suppose I had better keep the append-style for leakage traces?  :(
+    Is it still worthwhile to split up the io trace and leakage trace then?
+    I think so.
+    It still should be less of a pain to deal with them if they're separated.
+   *)
+  Inductive exec {pick_sp : PickSp} :
+    cmd -> trace -> io_trace -> mem -> locals -> metrics ->
     (trace -> io_trace -> mem -> locals -> metrics -> Prop) -> Prop :=
   | skip
-    pick_sp k t m l mc post
+    k t m l mc post
     (_ : post k t m l mc)
-    : exec pick_sp cmd.skip k t m l mc post
+    : exec cmd.skip k t m l mc post
   | set x e
-    pick_sp m l mc post
-    k t v mc' k' (_ : eval_expr m l e mc nil = Some (v, mc', k'))
-    (_ : post (k' ++ k) t m (map.put l x v) (addMetricInstructions 1
+    m l mc post
+    k t v mc' k' (_ : eval_expr m l e mc k = Some (v, mc', k'))
+    (_ : post k' t m (map.put l x v) (addMetricInstructions 1
                                       (addMetricLoads 1 mc')))
-    : exec pick_sp (cmd.set x e) k t m l mc post
+    : exec (cmd.set x e) k t m l mc post
   | unset x
-    pick_sp k t m l mc post
+    k t m l mc post
     (_ : post k t m (map.remove l x) mc)
-    : exec pick_sp (cmd.unset x) k t m l mc post
+    : exec (cmd.unset x) k t m l mc post
   | store sz ea ev
-    pick_sp k t m l mc post
-    a mc' k' (_ : eval_expr m l ea mc nil = Some (a, mc', k'))
-    v mc'' k'' (_ : eval_expr m l ev mc' nil = Some (v, mc'', k''))
+    k t m l mc post
+    a mc' k' (_ : eval_expr m l ea mc k = Some (a, mc', k'))
+    v mc'' k'' (_ : eval_expr m l ev mc' k' = Some (v, mc'', k''))
     m' (_ : store sz m a v = Some m')
-    (_ : post (leak_word a :: k'' ++ k' ++ k) t m' l (addMetricInstructions 1
-                                                        (addMetricLoads 1
-                                                           (addMetricStores 1 mc''))))
-    : exec pick_sp (cmd.store sz ea ev) k t m l mc post
+    (_ : post (leak_word a :: k'') t m' l (addMetricInstructions 1
+                                             (addMetricLoads 1
+                                                (addMetricStores 1 mc''))))
+    : exec (cmd.store sz ea ev) k t m l mc post
   | stackalloc x n body
-    pick_sp k t mSmall l mc post
+    k t mSmall l mc post
     (_ : Z.modulo n (bytes_per_word width) = 0)
     (_ : forall mStack mCombined,
-        let a := pick_sp nil in
+        let a := pick_sp k in
         anybytes a n mStack ->
         map.split mCombined mSmall mStack ->
-        exec pick_sp body k t mCombined (map.put l x a) (addMetricInstructions 1 (addMetricLoads 1 mc))
+        exec body k t mCombined (map.put l x a) (addMetricInstructions 1 (addMetricLoads 1 mc))
           (fun k' t' mCombined' l' mc' =>
              exists mSmall' mStack',
               anybytes a n mStack' /\
               map.split mCombined' mSmall' mStack' /\
               post k' t' mSmall' l' mc'))
-    : exec pick_sp (cmd.stackalloc x n body) k t mSmall l mc post
+    : exec (cmd.stackalloc x n body) k t mSmall l mc post
   | if_true k t m l mc e c1 c2 post
-    pick_sp v mc' k' (_ : eval_expr m l e mc nil = Some (v, mc', k'))
+    v mc' k' (_ : eval_expr m l e mc k = Some (v, mc', k'))
     (_ : word.unsigned v <> 0)
-    (_ : exec (fun k => pick_sp (k ++ leak_bool true :: k')) c1 (leak_bool true :: k' ++ k) t m l (addMetricInstructions 2 (addMetricLoads 2 (addMetricJumps 1 mc'))) post)
-    : exec pick_sp (cmd.cond e c1 c2) k t m l mc post
+    (_ : exec c1 (leak_bool true :: k') t m l (addMetricInstructions 2 (addMetricLoads 2 (addMetricJumps 1 mc'))) post)
+    : exec (cmd.cond e c1 c2) k t m l mc post
   | if_false e c1 c2
-    pick_sp k t m l mc post
-    v mc' k' (_ : eval_expr m l e mc nil = Some (v, mc', k'))
+    k t m l mc post
+    v mc' k' (_ : eval_expr m l e mc k = Some (v, mc', k'))
     (_ : word.unsigned v = 0)
-    (_ : exec (fun k => pick_sp (k ++ leak_bool false :: k')) c2 (leak_bool false :: k' ++ k) t m l (addMetricInstructions 2 (addMetricLoads 2 (addMetricJumps 1 mc'))) post)
-    : exec pick_sp (cmd.cond e c1 c2) k t m l mc post
+    (_ : exec c2 (leak_bool false :: k') t m l (addMetricInstructions 2 (addMetricLoads 2 (addMetricJumps 1 mc'))) post)
+    : exec (cmd.cond e c1 c2) k t m l mc post
   | seq c1 c2
-    k t m l mc pick_sp post
-    mid (_ : exec pick_sp c1 k t m l mc mid)
-    (_ : forall k' t' m' l' mc',
-        mid k' t' m' l' mc' ->
-        exec (fun k0 => pick_sp (k0 ++ firstn (length k' - length k) k')) c2 k' t' m' l' mc' post)
-    : exec pick_sp (cmd.seq c1 c2) k t m l mc post
+    k t m l mc post
+    mid (_ : exec c1 k t m l mc mid)
+    (_ : forall k' t' m' l' mc', mid k' t' m' l' mc' -> exec c2 k' t' m' l' mc' post)
+    : exec (cmd.seq c1 c2) k t m l mc post
   | while_false e c
-    pick_sp k t m l mc post
-    v mc' k' (_ : eval_expr m l e mc nil = Some (v, mc', k'))
+    k t m l mc post
+    v mc' k' (_ : eval_expr m l e mc k = Some (v, mc', k'))
     (_ : word.unsigned v = 0)
-    (_ : post (leak_bool false :: k' ++ k) t m l (addMetricInstructions 1
-                                                    (addMetricLoads 1
-                                                       (addMetricJumps 1 mc'))))
-    : exec pick_sp (cmd.while e c) k t m l mc post
+    (_ : post (leak_bool false :: k') t m l (addMetricInstructions 1
+                                                (addMetricLoads 1
+                                                   (addMetricJumps 1 mc'))))
+    : exec (cmd.while e c) k t m l mc post
   | while_true e c
-      pick_sp k t m l mc post
-      v mc' k' (_ : eval_expr m l e mc nil = Some (v, mc', k'))
+      k t m l mc post
+      v mc' k' (_ : eval_expr m l e mc k = Some (v, mc', k'))
       (_ : word.unsigned v <> 0)
-      mid (_ : exec (fun k0 => pick_sp (k0 ++ leak_bool true :: k')) c (leak_bool true :: k' ++ k) t m l mc' mid)
-      (_ : forall k'' t' m' l' mc'',
-          mid k'' t' m' l' mc'' ->
-          exec (fun k0 => pick_sp (k0 ++ firstn (length k'' - length k) k'')) (cmd.while e c) k'' t' m' l' (addMetricInstructions 2
-                                                                                                              (addMetricLoads 2
-                                                                                                                 (addMetricJumps 1 mc''))) post)
-    : exec pick_sp (cmd.while e c) k t m l mc post
+      mid (_ : exec c (leak_bool true :: k') t m l mc' mid)
+      (_ : forall k'' t' m' l' mc'', mid k'' t' m' l' mc'' ->
+                                      exec (cmd.while e c) k'' t' m' l' (addMetricInstructions 2
+                                                                           (addMetricLoads 2
+                                                                              (addMetricJumps 1 mc''))) post)
+    : exec (cmd.while e c) k t m l mc post
   | call binds fname arges
-      pick_sp k t m l mc post
+      k t m l mc post
       params rets fbody (_ : map.get e fname = Some (params, rets, fbody))
-      args mc' k' (_ : evaluate_call_args_log m l arges mc nil = Some (args, mc', k'))
+      args mc' k' (_ : evaluate_call_args_log m l arges mc k = Some (args, mc', k'))
       lf (_ : map.of_list_zip params args = Some lf)
-      mid (_ : exec (fun k0 => pick_sp (k0 ++ leak_unit :: k')) fbody (leak_unit :: k' ++ k) t m lf (addMetricInstructions 100 (addMetricJumps 100 (addMetricLoads 100 (addMetricStores 100 mc')))) mid)
+      mid (_ : exec fbody (leak_unit :: k') t m lf (addMetricInstructions 100 (addMetricJumps 100 (addMetricLoads 100 (addMetricStores 100 mc')))) mid)
       (_ : forall k'' t' m' st1 mc'', mid k'' t' m' st1 mc'' ->
           exists retvs, map.getmany_of_list st1 rets = Some retvs /\
           exists l', map.putmany_of_list_zip binds retvs l = Some l' /\
           post k'' t' m' l' (addMetricInstructions 100 (addMetricJumps 100 (addMetricLoads 100 (addMetricStores 100 mc'')))))
-    : exec pick_sp (cmd.call binds fname arges) k t m l mc post
+    : exec (cmd.call binds fname arges) k t m l mc post
   | interact binds action arges
-      pick_sp k t m l mc post
+      k t m l mc post
       mKeep mGive (_: map.split m mKeep mGive)
-      args mc' k' (_ :  evaluate_call_args_log m l arges mc nil = Some (args, mc', k'))
+      args mc' k' (_ :  evaluate_call_args_log m l arges mc k = Some (args, mc', k'))
       mid (_ : ext_spec t mGive action args mid)
       (_ : forall mReceive resvals klist, mid mReceive resvals klist ->
           exists l', map.putmany_of_list_zip binds resvals l = Some l' /\
           forall m', map.split m' mKeep mReceive ->
-          post (leak_list klist :: k' ++ k)%list (((mGive, action, args), (mReceive, resvals)) :: t) m' l'
+          post (leak_list klist :: k')%list (((mGive, action, args), (mReceive, resvals)) :: t) m' l'
             (addMetricInstructions 1
                (addMetricStores 1
                   (addMetricLoads 2 mc'))))
-    : exec pick_sp (cmd.interact binds action arges) k t m l mc post
+    : exec (cmd.interact binds action arges) k t m l mc post
   .
   
   Context {word_ok: word.ok word} {mem_ok: map.ok mem} {ext_spec_ok: ext_spec.ok ext_spec}.
 
-  Lemma weaken : forall pick_sp s k t m l mc post1,
-      exec pick_sp s k t m l mc post1 ->
+  Lemma weaken {pick_sp: PickSp} : forall s k t m l mc post1,
+      exec s k t m l mc post1 ->
       forall post2: _ -> _ -> _ -> _ -> _ -> Prop,
         (forall k' t' m' l' mc', post1 k' t' m' l' mc' -> post2 k' t' m' l' mc') ->
-        exec pick_sp s k t m l mc post2.
+        exec s k t m l mc post2.
   Proof.
     induction 1; intros; try solve [econstructor; eauto].
     - eapply stackalloc. 1: assumption.
@@ -420,16 +439,16 @@ Module exec. Section WithEnv.
       eauto 10.
   Qed.
 
-  Lemma intersect : forall pick_sp k t l m mc s post1,
-      exec pick_sp s k t m l mc post1 ->
+  Lemma intersect {pick_sp: PickSp} : forall k t l m mc s post1,
+      exec s k t m l mc post1 ->
       forall post2,
-        exec pick_sp s k t m l mc post2 ->
-        exec pick_sp s k t m l mc (fun k' t' m' l' mc' => post1 k' t' m' l' mc' /\ post2 k' t' m' l' mc').
+        exec s k t m l mc post2 ->
+        exec s k t m l mc (fun k' t' m' l' mc' => post1 k' t' m' l' mc' /\ post2 k' t' m' l' mc').
   Proof.
     induction 1;
       intros;
       match goal with
-      | H: exec _ _ _ _ _ _ _ _ |- _ => inversion H; subst; clear H
+      | H: exec _ _ _ _ _ _ _ |- _ => inversion H; subst; clear H
       end;
       repeat match goal with
              | H1: ?e = Some (?v1, ?mc1, ?t1), H2: ?e = Some (?v2, ?mc2, ?t2) |- _ =>
@@ -661,4 +680,405 @@ Module exec. Section WithEnv.
       
   End WithEnv.
 End exec. Notation exec := exec.exec.
+
+Module otherexec. Section WithEnv.
+  Context {width: Z} {BW: Bitwidth width} {word: word.word width} {mem: map.map word byte}.
+  Context {locals: map.map String.string word}.
+  Context {env: map.map String.string (list String.string * list String.string * cmd)}.
+  Context {ext_spec: ExtSpec}.
+  Context (e: env).
+
+  Local Notation metrics := MetricLog.
+
+  Implicit Types post : trace -> io_trace -> mem -> locals -> metrics -> Prop. (* COQBUG(unification finds Type instead of Prop and fails to downgrade *)
+
+  (*maybe input trace should be entire trace so far, but trace in postcondition should just be trace accumulated during execution.*)
+  Inductive exec :
+    (trace -> word) -> cmd -> trace -> io_trace -> mem -> locals -> metrics ->
+    (trace -> io_trace -> mem -> locals -> metrics -> Prop) -> Prop :=
+  | skip
+    pick_sp k t m l mc post
+    (_ : post k t m l mc)
+    : exec pick_sp cmd.skip k t m l mc post
+  | set x e
+    pick_sp m l mc post
+    k t v mc' k' (_ : eval_expr m l e mc nil = Some (v, mc', k'))
+    (_ : post (k' ++ k) t m (map.put l x v) (addMetricInstructions 1
+                                      (addMetricLoads 1 mc')))
+    : exec pick_sp (cmd.set x e) k t m l mc post
+  | unset x
+    pick_sp k t m l mc post
+    (_ : post k t m (map.remove l x) mc)
+    : exec pick_sp (cmd.unset x) k t m l mc post
+  | store sz ea ev
+    pick_sp k t m l mc post
+    a mc' k' (_ : eval_expr m l ea mc nil = Some (a, mc', k'))
+    v mc'' k'' (_ : eval_expr m l ev mc' nil = Some (v, mc'', k''))
+    m' (_ : store sz m a v = Some m')
+    (_ : post (leak_word a :: k'' ++ k' ++ k) t m' l (addMetricInstructions 1
+                                                        (addMetricLoads 1
+                                                           (addMetricStores 1 mc''))))
+    : exec pick_sp (cmd.store sz ea ev) k t m l mc post
+  | stackalloc x n body
+    pick_sp k t mSmall l mc post
+    (_ : Z.modulo n (bytes_per_word width) = 0)
+    (_ : forall mStack mCombined,
+        let a := pick_sp nil in
+        anybytes a n mStack ->
+        map.split mCombined mSmall mStack ->
+        exec pick_sp body k t mCombined (map.put l x a) (addMetricInstructions 1 (addMetricLoads 1 mc))
+          (fun k' t' mCombined' l' mc' =>
+             exists mSmall' mStack',
+              anybytes a n mStack' /\
+              map.split mCombined' mSmall' mStack' /\
+              post k' t' mSmall' l' mc'))
+    : exec pick_sp (cmd.stackalloc x n body) k t mSmall l mc post
+  | if_true k t m l mc e c1 c2 post
+    pick_sp v mc' k' (_ : eval_expr m l e mc nil = Some (v, mc', k'))
+    (_ : word.unsigned v <> 0)
+    (_ : exec (fun k => pick_sp (k ++ leak_bool true :: k')) c1 (leak_bool true :: k' ++ k) t m l (addMetricInstructions 2 (addMetricLoads 2 (addMetricJumps 1 mc'))) post)
+    : exec pick_sp (cmd.cond e c1 c2) k t m l mc post
+  | if_false e c1 c2
+    pick_sp k t m l mc post
+    v mc' k' (_ : eval_expr m l e mc nil = Some (v, mc', k'))
+    (_ : word.unsigned v = 0)
+    (_ : exec (fun k => pick_sp (k ++ leak_bool false :: k')) c2 (leak_bool false :: k' ++ k) t m l (addMetricInstructions 2 (addMetricLoads 2 (addMetricJumps 1 mc'))) post)
+    : exec pick_sp (cmd.cond e c1 c2) k t m l mc post
+  | seq c1 c2
+    k t m l mc pick_sp post
+    mid (_ : exec pick_sp c1 k t m l mc mid)
+    (_ : forall k' t' m' l' mc',
+        mid k' t' m' l' mc' ->
+        exec (fun k0 => pick_sp (k0 ++ firstn (length k' - length k) k')) c2 k' t' m' l' mc' post)
+    : exec pick_sp (cmd.seq c1 c2) k t m l mc post
+  | while_false e c
+    pick_sp k t m l mc post
+    v mc' k' (_ : eval_expr m l e mc nil = Some (v, mc', k'))
+    (_ : word.unsigned v = 0)
+    (_ : post (leak_bool false :: k' ++ k) t m l (addMetricInstructions 1
+                                                    (addMetricLoads 1
+                                                       (addMetricJumps 1 mc'))))
+    : exec pick_sp (cmd.while e c) k t m l mc post
+  | while_true e c
+      pick_sp k t m l mc post
+      v mc' k' (_ : eval_expr m l e mc nil = Some (v, mc', k'))
+      (_ : word.unsigned v <> 0)
+      mid (_ : exec (fun k0 => pick_sp (k0 ++ leak_bool true :: k')) c (leak_bool true :: k' ++ k) t m l mc' mid)
+      (_ : forall k'' t' m' l' mc'',
+          mid k'' t' m' l' mc'' ->
+          exec (fun k0 => pick_sp (k0 ++ firstn (length k'' - length k) k'')) (cmd.while e c) k'' t' m' l' (addMetricInstructions 2
+                                                                                                              (addMetricLoads 2
+                                                                                                                 (addMetricJumps 1 mc''))) post)
+    : exec pick_sp (cmd.while e c) k t m l mc post
+  | call binds fname arges
+      pick_sp k t m l mc post
+      params rets fbody (_ : map.get e fname = Some (params, rets, fbody))
+      args mc' k' (_ : evaluate_call_args_log m l arges mc nil = Some (args, mc', k'))
+      lf (_ : map.of_list_zip params args = Some lf)
+      mid (_ : exec (fun k0 => pick_sp (k0 ++ leak_unit :: k')) fbody (leak_unit :: k' ++ k) t m lf (addMetricInstructions 100 (addMetricJumps 100 (addMetricLoads 100 (addMetricStores 100 mc')))) mid)
+      (_ : forall k'' t' m' st1 mc'', mid k'' t' m' st1 mc'' ->
+          exists retvs, map.getmany_of_list st1 rets = Some retvs /\
+          exists l', map.putmany_of_list_zip binds retvs l = Some l' /\
+          post k'' t' m' l' (addMetricInstructions 100 (addMetricJumps 100 (addMetricLoads 100 (addMetricStores 100 mc'')))))
+    : exec pick_sp (cmd.call binds fname arges) k t m l mc post
+  | interact binds action arges
+      pick_sp k t m l mc post
+      mKeep mGive (_: map.split m mKeep mGive)
+      args mc' k' (_ :  evaluate_call_args_log m l arges mc nil = Some (args, mc', k'))
+      mid (_ : ext_spec t mGive action args mid)
+      (_ : forall mReceive resvals klist, mid mReceive resvals klist ->
+          exists l', map.putmany_of_list_zip binds resvals l = Some l' /\
+          forall m', map.split m' mKeep mReceive ->
+          post (leak_list klist :: k' ++ k)%list (((mGive, action, args), (mReceive, resvals)) :: t) m' l'
+            (addMetricInstructions 1
+               (addMetricStores 1
+                  (addMetricLoads 2 mc'))))
+    : exec pick_sp (cmd.interact binds action arges) k t m l mc post
+  .
+  
+  Context {word_ok: word.ok word} {mem_ok: map.ok mem} {ext_spec_ok: ext_spec.ok ext_spec}.
+
+  Lemma weaken : forall pick_sp s k t m l mc post1,
+      exec pick_sp s k t m l mc post1 ->
+      forall post2: _ -> _ -> _ -> _ -> _ -> Prop,
+        (forall k' t' m' l' mc', post1 k' t' m' l' mc' -> post2 k' t' m' l' mc') ->
+        exec pick_sp s k t m l mc post2.
+  Proof.
+    induction 1; intros; try solve [econstructor; eauto].
+    - eapply stackalloc. 1: assumption.
+      intros.
+      eapply H1; eauto.
+      intros. fwd. eauto 10.
+    - eapply call.
+      4: eapply IHexec.
+      all: eauto.
+      intros.
+      edestruct H3 as (? & ? & ? & ? & ?); [eassumption|].
+      eauto 10.
+    - eapply interact; try eassumption.
+      intros.
+      edestruct H2 as (? & ? & ?); [eassumption|].
+      eauto 10.
+  Qed.
+
+  Lemma intersect : forall pick_sp k t l m mc s post1,
+      exec pick_sp s k t m l mc post1 ->
+      forall post2,
+        exec pick_sp s k t m l mc post2 ->
+        exec pick_sp s k t m l mc (fun k' t' m' l' mc' => post1 k' t' m' l' mc' /\ post2 k' t' m' l' mc').
+  Proof.
+    induction 1;
+      intros;
+      match goal with
+      | H: exec _ _ _ _ _ _ _ _ |- _ => inversion H; subst; clear H
+      end;
+      repeat match goal with
+             | H1: ?e = Some (?v1, ?mc1, ?t1), H2: ?e = Some (?v2, ?mc2, ?t2) |- _ =>
+               replace v2 with v1 in * by congruence;
+               replace mc2 with mc1 in * by congruence;
+               replace t2 with t1 in * by congruence; clear v2 mc2 t2 H2
+             end;
+      repeat match goal with
+             | H1: ?e = Some ?v1, H2: ?e = Some ?v2 |- _ =>
+               replace v2 with v1 in * by congruence; clear H2
+             end;
+      try solve [econstructor; eauto | exfalso; congruence].
+    
+    - econstructor. 1: eassumption.
+      intros.
+      rename H0 into Ex1, H14 into Ex2.
+      eapply weaken. 1: eapply H1. 1,2: eassumption.
+      1: eapply Ex2. 1,2: eassumption.
+      cbv beta.
+      intros. fwd.
+      lazymatch goal with
+      | A: map.split _ _ _, B: map.split _ _ _ |- _ =>
+        specialize @map.split_diff with (4 := A) (5 := B) as P
+      end.
+      edestruct P; try typeclasses eauto. 2: subst; eauto 10.
+      eapply anybytes_unique_domain; eassumption.
+    - econstructor.
+      + eapply IHexec. exact H6. (* not H *)
+      + simpl. intros *. intros [? ?]. eauto.
+    - eapply while_true. 1, 2: eassumption.
+      + eapply IHexec. exact H10. (* not H1 *)
+      + simpl. intros *. intros [? ?]. eauto.
+    - eapply call. 1, 2, 3: eassumption.
+      + eapply IHexec. exact H18. (* not H2 *)
+      + simpl. intros *. intros [? ?].
+        edestruct H3 as (? & ? & ? & ? & ?); [eassumption|].
+        edestruct H19 as (? & ? & ? & ? & ?); [eassumption|].
+        repeat match goal with
+               | H1: ?e = Some ?v1, H2: ?e = Some ?v2 |- _ =>
+                 replace v2 with v1 in * by congruence; clear H2
+               end.
+        eauto 10.
+    - pose proof ext_spec.unique_mGive_footprint as P.
+      specialize P with (1 := H1) (2 := H16).
+      destruct (map.split_diff P H H7). subst mKeep0 mGive0. clear H7.
+      eapply interact. 1,2: eassumption.
+      + eapply ext_spec.intersect; [ exact H1 | exact H16 ].
+      + simpl. intros *. intros [? ?].
+        edestruct H2 as (? & ? & ?); [eassumption|].
+        edestruct H17 as (? & ? & ?); [eassumption|].
+        repeat match goal with
+               | H1: ?e = Some ?v1, H2: ?e = Some ?v2 |- _ =>
+                 replace v2 with v1 in * by congruence; clear H2
+               end.
+        eauto 10.
+  Qed.
+
+  Require Import coqutil.Z.Lia.
+
+  Lemma eval_expr_extends_trace :
+    forall e0 m l mc k v mc' k',
+    eval_expr m l e0 mc k = Some (v, mc', k') ->
+    exists k'', k' = k'' ++ k.
+  Proof.
+    intros e0. induction e0; intros; simpl in *;
+      repeat match goal with
+        | H: (let (_, _) := ?x in _) = _ |- _ =>
+            destruct x
+        | H: match ?x with
+             | Some _ => _
+             | None => _
+             end = Some (_, _, _) |- _ =>
+            destruct x eqn:?; try congruence
+        | H: Some (?v1, ?mc1, ?t1) = Some (?v2, ?mc2, ?t2) |- _ =>
+            injection H; intros; subst
+        end.
+    - eexists. trace_alignment.
+    - eexists. trace_alignment.
+    - specialize IHe0 with (1 := Heqo). fwd. eexists. trace_alignment.
+    - specialize IHe0 with (1 := Heqo). fwd. eexists. trace_alignment.
+    - specialize IHe0_1 with (1 := Heqo). specialize IHe0_2 with (1 := Heqo0). fwd.
+      eexists. trace_alignment.
+    - specialize IHe0_1 with (1 := Heqo). destruct (word.eqb _ _).
+      + specialize IHe0_3 with (1 := H). fwd. eexists. trace_alignment.
+      + specialize IHe0_2 with (1 := H). fwd. eexists. trace_alignment.
+  Qed.
+
+  Lemma evaluate_call_args_log_extends_trace :
+    forall arges m l mc k args mc' k',
+    evaluate_call_args_log m l arges mc k = Some (args, mc', k') ->
+    exists k'', k' = k'' ++ k.
+  Proof.
+    intros arges. induction arges.
+    - simpl. intros. injection H. intros. subst. eexists. trace_alignment.
+    - simpl. intros. destruct (eval_expr _ _ _ _ _) eqn:E1; try congruence.
+      destruct p. destruct p. destruct (evaluate_call_args_log _ _ _ _ _) eqn:E2; try congruence.
+      destruct p. destruct p. injection H. intros. subst.
+      apply eval_expr_extends_trace in E1. specialize IHarges with (1 := E2).
+      fwd. eexists. trace_alignment.
+  Qed.
+
+  Local Ltac subst_exprs :=
+    repeat match goal with
+      | H : eval_expr _ _ _ _ _ = Some _ |- _ =>
+          apply eval_expr_extends_trace in H; destruct H; subst
+      | H : evaluate_call_args_log _ _ _ _ _ = Some _ |- _ =>
+          apply evaluate_call_args_log_extends_trace in H; destruct H; subst
+        end.
+
+  Lemma exec_extends_trace pick_sp s k t m l mc post :
+    exec pick_sp s k t m l mc post ->
+    exec pick_sp s k t m l mc (fun k' t' m' l' mc' => post k' t' m' l' mc' /\ exists k'', k' = k'' ++ k).
+  Proof.
+    intros H. induction H; try (econstructor; intuition eauto; subst_exprs; eexists; trace_alignment; fail).
+    - econstructor; intuition eauto. intros. eapply weaken. 1: eapply H1; eauto.
+      simpl. intros. fwd. eexists. eexists. intuition eauto.
+    - eapply if_true; intuition eauto. eapply weaken. 1: eapply IHexec.
+      simpl. intros. fwd. intuition eauto. subst_exprs. eexists. trace_alignment.
+    - eapply if_false; intuition eauto. eapply weaken. 1: eapply IHexec.
+      simpl. intros. fwd. intuition eauto. subst_exprs. eexists. trace_alignment.
+    - econstructor; intuition eauto. fwd. eapply weaken. 1: eapply H1; eauto.
+      simpl. intros. fwd. intuition eauto. eexists. trace_alignment.
+    - eapply while_true; eauto. simpl. intros. fwd. eapply weaken. 1: eapply H3; eauto.
+      simpl. intros. fwd. intuition eauto. subst_exprs. eexists. trace_alignment.
+    - econstructor; intuition eauto. fwd. specialize H3 with (1 := H4p0). fwd.
+      eexists. intuition eauto. eexists. intuition eauto. subst_exprs.
+      eexists. trace_alignment.
+    - econstructor; intuition eauto. specialize H2 with (1 := H3). fwd.
+      eexists. intuition eauto. subst_exprs. eexists. trace_alignment.
+  Qed.
+
+  (*Lemma exec_ext pick_sp1 s k t m l mc post :
+    exec pick_sp1 s k t m l mc post ->
+    forall pick_sp2,
+    (forall k', pick_sp1 k' = pick_sp2 k') ->
+    exec pick_sp2 s k t m l mc post.
+  Proof.
+    Set Printing Implicit.
+    intros H1 pick_sp2. induction H1; intros; try solve [econstructor; eauto].
+    - econstructor; eauto. intros. replace (pick_sp nil) with (pick_sp2 nil) in *.
+      { subst a. eapply weaken. 1: eapply H1; eauto. simpl. eauto. }
+      symmetry. apply H2 with (k' := nil).
+    - eapply if_true; eauto. eapply IHexec. subst_exprs.
+      intros. eassert (H2' := H2 (_ ++ _ :: _)). rewrite <- app_assoc in H2'. eapply H2'.
+    - eapply if_false; eauto. eapply IHexec. subst_exprs.
+      intros. eassert (H2' := H2 (_ ++ _ :: _)). rewrite <- app_assoc in H2'. eapply H2'.
+    - econstructor. 1: eapply exec_extends_trace; eauto. simpl. intros. fwd.
+      eapply H0; eauto. intros. repeat rewrite app_assoc. apply H2.
+    - eapply while_true; intuition eauto.
+      { eapply exec_extends_trace. eapply IHexec. subst_exprs.
+        intros. repeat (rewrite app_assoc || rewrite (app_one_l _ (_ ++ k))). auto. }
+      simpl in *. fwd. eapply H3; eauto. intros. subst_exprs.
+      repeat (rewrite app_assoc || rewrite (app_one_l _ (_ ++ k))). auto.
+    - econstructor. 4: eapply exec_extends_trace. all: intuition eauto.
+      { eapply IHexec. subst_exprs. intros.
+        repeat (rewrite app_assoc || rewrite (app_one_l _ (_ ++ k))). auto. }
+      fwd. specialize H3 with (1 := H5p0). fwd. intuition eauto.
+  Qed.*)
+  
+  Local Ltac solve_picksps_equal :=
+    intros; cbv beta; f_equal;
+    repeat (rewrite rev_app_distr || cbn [rev app]); rewrite List.skipn_app_r;
+    [|repeat (rewrite app_length || rewrite rev_length || simpl); blia];
+    repeat rewrite <- app_assoc; rewrite List.skipn_app_r;
+    [|rewrite rev_length; reflexivity];
+    repeat (rewrite rev_app_distr || cbn [rev app] || rewrite rev_involutive);
+    repeat rewrite <- app_assoc; reflexivity.
+
+  (*Lemma exec_to_other_trace (pick_sp: PickSp) s k1 k2 t m l mc post :
+    exec s k1 t m l mc post ->
+    exec (pick_sp := fun k => pick_sp (rev (skipn (length k2) (rev k)) ++ k1))
+      s k2 t m l mc (fun k2' t' m' l' mc' =>
+                       exists k'',
+                         k2' = k'' ++ k2 /\
+                           post (k'' ++ k1) t' m' l' mc').
+  Proof.
+    intros H. generalize dependent k2. induction H; intros.
+    - econstructor. exists nil. eauto.
+    - apply expr_to_other_trace in H. destruct H as [k'' [H1 H2] ]. subst.
+      econstructor; intuition eauto.
+    - econstructor; intuition. exists nil. intuition.
+    - apply expr_to_other_trace in H. apply expr_to_other_trace in H0.
+      destruct H as [k''a [H3 H4] ]. subst. destruct H0 as [k''v [H5 H6] ]. subst.
+      econstructor; intuition eauto. eexists (_ :: _ ++ _). simpl.
+      repeat rewrite <- (app_assoc _ _ k2). repeat rewrite <- (app_assoc _ _ k).
+      intuition.
+    - econstructor; intuition. intros.
+      replace (rev k2) with (rev k2 ++ nil) in * by apply app_nil_r. Search (length (rev _)).
+      rewrite List.skipn_app_r in * by (rewrite rev_length; reflexivity).
+      simpl in *. eapply weaken. 1: eapply H1; eauto.
+      simpl. intros. fwd. exists mSmall', mStack'. intuition. eauto.
+    - apply expr_to_other_trace in H. fwd. eapply if_true; intuition eauto.
+      eapply weaken.
+      { eapply exec_ext with (pick_sp1 := _). 1: eapply IHexec. solve_picksps_equal. }
+      simpl. intros. fwd. eexists (_ ++ _ :: _).
+      repeat rewrite <- (app_assoc _ _ k2). repeat rewrite <- (app_assoc _ _ k).
+      intuition.
+    - apply expr_to_other_trace in H. fwd. eapply if_false; intuition.
+      eapply weaken.
+      { eapply exec_ext with (pick_sp1 := _). 1: eapply IHexec. solve_picksps_equal. }
+      simpl. intros. fwd. eexists (_ ++ _ :: _).
+      repeat rewrite <- (app_assoc _ _ k2). repeat rewrite <- (app_assoc _ _ k).
+      intuition.
+    - econstructor; intuition. fwd. eapply weaken.
+      { eapply exec_ext with (pick_sp1 := _). 1: eapply H1; eauto. solve_picksps_equal. }
+      simpl. intros. fwd. eexists (_ ++ _).
+      repeat rewrite <- (app_assoc _ _ k2). repeat rewrite <- (app_assoc _ _ k).
+      intuition.
+    - apply expr_to_other_trace in H. fwd. eapply while_false; intuition.
+      eexists (_ :: _). intuition.
+    - apply expr_to_other_trace in H. fwd. eapply while_true; intuition.
+      { eapply exec_ext with (pick_sp1 := _). 1: eapply IHexec. solve_picksps_equal. }
+      cbv beta in *. fwd. eapply weaken.
+      { eapply exec_ext with (pick_sp1 := _). 1: eapply H3; eauto. solve_picksps_equal. }
+      simpl. intros. fwd. eexists (_ ++ _ ++ _ :: _).
+      repeat rewrite <- (app_assoc _ _ k2). repeat rewrite <- (app_assoc _ _ k).
+      intuition.
+    - apply call_args_to_other_trace in H0.
+      fwd. econstructor; intuition eauto.
+      { eapply exec_ext with (pick_sp1 := _). 1: eapply IHexec; eauto. solve_picksps_equal. }
+      cbv beta in *. fwd. apply H3 in H0p2.
+      fwd. exists retvs. intuition. exists l'. intuition. eexists (_ ++ _ :: _).
+      repeat rewrite <- (app_assoc _ _ k2). repeat rewrite <- (app_assoc _ _ k).
+      intuition.
+    - apply call_args_to_other_trace in H0. fwd. econstructor; intuition eauto.
+      apply H2 in H0. fwd. exists l'. intuition. eexists (_ :: _).
+      intuition.
+  Qed.*)
+      
+  End WithEnv.
+End otherexec. Notation otherexec := otherexec.exec.
+
+Module twoexecs. Section WithEnv.
+  Context {width: Z} {BW: Bitwidth width} {word: word.word width} {mem: map.map word byte}.
+  Context {locals: map.map String.string word}.
+  Context {env: map.map String.string (list String.string * list String.string * cmd)}.
+  Context {ext_spec: ExtSpec}.
+  Context (e: env).
+
+  Local Notation metrics := MetricLog.
+
+  Implicit Types post : trace -> io_trace -> mem -> locals -> metrics -> Prop. (* COQBUG(unification finds Type instead of Prop and fails to downgrade *) Check exec.
+
+  Lemma global_to_local pick_sp s k t m l mc post :
+    exec e (pick_sp := pick_sp) s k t m l mc post ->
+    otherexec e pick_sp s k t m l mc post.
+  Proof.
+    intros H. induction H; try solve [econstructor; eauto].
+    - econstructor; eauto. econstructor; auto.
+     
 
